rupicola/io/Compilation.fst
@@ -5,7 +5,8 @@ open FStar.Tactics
 open STLC
 open QTyp
 open QExp
-open ExpRel
+open LogRelSourceTarget
+module C1 = LogRelSourceTarget.CompatibilityLemmas
 
 let rec compile #g #a (#s:fs_oval g a) (qs:g ⊢ s) : Tot exp (decreases qs) =
   match qs with
@@ -38,105 +39,121 @@ and compile_oprod #g #a (#s:fs_oprod g a) (qs:oprod_quotation g s) : Tot exp (de
   | QIfProd qc qt qe -> EIf (compile qc) (compile_oprod qt) (compile_oprod qe)
   | QCaseProd qcond qinlc qinrc -> ECase (compile qcond) (compile_oprod qinlc) (compile_oprod qinrc)
 
-let lem_compile_empty_closed #a (#s:fs_oval empty a) (qs:empty ⊢ s) : Lemma (is_closed (compile qs)) = admit ()
-
-let compile_closed  #a #s (qs:a ⊩ s) : closed_exp =
-  lem_compile_empty_closed qs;
-  compile qs
-
-let rec compile_equiv #g (#a:qType) (#s:fs_oval g a) (qs:g ⊢ s)
-  : Lemma (ensures (s ≈ (compile qs)))
+let rec lem_compile_equiv #g (#a:qType) (#s:fs_oval g a) (qs:g ⊢ s)
+  : Lemma (ensures (s ≈ (compile qs))) (decreases qs)
   = match qs with
-  | Qtt -> equiv_unit g
-  | QVar0 #g' #_ -> equiv_var0 g' a
+  | Qtt -> C1.equiv_oval_unit g
+  | QVar0 #g' #_ -> C1.equiv_oval_var0 g' a
   | QVarS #g' #_ #b #x qx ->
-    compile_equiv qx;
-    equiv_varS #g' #a #b x (compile qx)
-  | QFd fd -> equiv_file_descr g fd
-  | QAppGhost -> equiv_unit g
+    lem_compile_equiv qx;
+    C1.equiv_varS #g' #a #b x (compile qx)
+  | QFd fd -> C1.equiv_oval_file_descr g fd
+  | QAppGhost -> C1.equiv_oval_unit g
   | QApp #_ #qa #qb #f #x qf qx ->
-    compile_equiv qf;
-    compile_equiv qx;
-    equiv_app f x (compile qf) (compile qx)
+    lem_compile_equiv qf;
+    lem_compile_equiv qx;
+    C1.equiv_oval_app f x (compile qf) (compile qx)
   | QLambda #_ #_ #_ #body qbody ->
-    compile_equiv qbody;
-    equiv_lam body (compile qbody)
-  | QFalse -> equiv_false g
-  | QTrue -> equiv_true g
+    lem_compile_equiv qbody;
+    C1.equiv_oval_lambda body (compile qbody)
+  | QFalse -> C1.equiv_oval_false g
+  | QTrue -> C1.equiv_oval_true g
   | QIf #_ #_ #c qc #t qt #e qe ->
-    compile_equiv qc;
-    compile_equiv qt;
-    compile_equiv qe;
-    equiv_if c t e (compile qc) (compile qt) (compile qe)
+    lem_compile_equiv qc;
+    lem_compile_equiv qt;
+    lem_compile_equiv qe;
+    C1.equiv_oval_if c t e (compile qc) (compile qt) (compile qe)
   | QMkpair #_ #a1 #a2 #s1 #s2 q1 q2 ->
-    compile_equiv q1;
-    compile_equiv q2;
-    equiv_pair s1 s2 (compile q1) (compile q2)
+    lem_compile_equiv q1;
+    lem_compile_equiv q2;
+    C1.equiv_oval_pair s1 s2 (compile q1) (compile q2)
   | QFst #_ #_ #_ #p qp ->
-    compile_equiv qp;
-    equiv_pair_fst_app p (compile qp)
+    lem_compile_equiv qp;
+    C1.equiv_oval_pair_fst_app p (compile qp)
   | QSnd #_ #_ #_ #p qp ->
-    compile_equiv qp;
-    equiv_pair_snd_app p (compile qp)
+    lem_compile_equiv qp;
+    C1.equiv_oval_pair_snd_app p (compile qp)
   | QInl #_ #_ #t2 #p qp ->
-    compile_equiv qp;
-    equiv_inl t2 p (compile qp)
+    lem_compile_equiv qp;
+    C1.equiv_oval_inl t2 p (compile qp)
   | QInr #_ #t1 #_ #p qp ->
-    compile_equiv qp;
-    equiv_inr t1 p (compile qp)
+    lem_compile_equiv qp;
+    C1.equiv_oval_inr t1 p (compile qp)
   | QCase #_ #_ #_ #_ #cond qcond #inlc qinlc #inrc qinrc ->
-    compile_equiv qcond;
-    compile_equiv qinlc;
-    compile_equiv qinrc;
-    equiv_case cond inlc inrc (compile qcond) (compile qinlc) (compile qinrc)
+    lem_compile_equiv qcond;
+    lem_compile_equiv qinlc;
+    lem_compile_equiv qinrc;
+    C1.equiv_oval_case cond inlc inrc (compile qcond) (compile qinlc) (compile qinrc)
   | QLambdaProd #_ #_ #_ #body qbody ->
-    compile_equiv_prod qbody;
-    equiv_lam_prod body (compile_oprod qbody)
-and compile_equiv_prod #g (#a:qType) (#s:fs_oprod g a) (qs:oprod_quotation g s)
+    lem_compile_equiv_prod qbody;
+    C1.equiv_oval_lambda_oprod body (compile_oprod qbody)
+and lem_compile_equiv_prod #g (#a:qType) (#s:fs_oprod g a) (qs:oprod_quotation g s)
   : Lemma (ensures (s ≋ (compile_oprod qs))) (decreases qs)
   =
   match qs with
   | QOpenfile #_ #fnm qfnm ->
-    compile_equiv qfnm;
-    equiv_oprod_openfile_oval fnm (compile qfnm)
+    lem_compile_equiv qfnm;
+    C1.equiv_oprod_openfile_oval fnm (compile qfnm)
   | QRead #_ #fd qfd ->
-    compile_equiv qfd;
-    equiv_oprod_read_oval fd (compile qfd)
+    lem_compile_equiv qfd;
+    C1.equiv_oprod_read_oval fd (compile qfd)
   | QWrite #_ #fd #msg qfd qmsg ->
-    compile_equiv qfd;
-    compile_equiv qmsg;
-    equiv_oprod_write_oval fd msg (compile qfd) (compile qmsg)
+    lem_compile_equiv qfd;
+    lem_compile_equiv qmsg;
+    C1.equiv_oprod_write_oval fd msg (compile qfd) (compile qmsg)
   | QClose #_ #fd qfd ->
-    compile_equiv qfd;
-    equiv_oprod_close_oval fd (compile qfd)
+    lem_compile_equiv qfd;
+    C1.equiv_oprod_close_oval fd (compile qfd)
   | QReturn #_ #_ #x qx ->
-    compile_equiv qx;
-    equiv_oprod_return x (compile qx)
+    lem_compile_equiv qx;
+    C1.equiv_oprod_return x (compile qx)
   | QBindProd #_ #_ #_ #m #k qm qk ->
-    compile_equiv_prod qm;
-    compile_equiv_prod qk;
-    equiv_oprod_bind m k (compile_oprod qm) (compile_oprod qk)
+    lem_compile_equiv_prod qm;
+    lem_compile_equiv_prod qk;
+    C1.equiv_oprod_bind m k (compile_oprod qm) (compile_oprod qk)
   | QAppProd #_ #_ #_ #f #x qf qx ->
-    compile_equiv qf;
-    compile_equiv qx;
-    equiv_oprod_app_oval_oval f x (compile qf) (compile qx)
+    lem_compile_equiv qf;
+    lem_compile_equiv qx;
+    C1.equiv_oprod_app_oval_oval f x (compile qf) (compile qx)
   | QIfProd #_ #_ #c qc #t qt #e qe ->
-    compile_equiv qc;
-    compile_equiv_prod qt;
-    compile_equiv_prod qe;
-    equiv_oprod_if_oval c t e (compile qc) (compile_oprod qt) (compile_oprod qe)
+    lem_compile_equiv qc;
+    lem_compile_equiv_prod qt;
+    lem_compile_equiv_prod qe;
+    C1.equiv_oprod_if_oval c t e (compile qc) (compile_oprod qt) (compile_oprod qe)
   | QCaseProd #_ #_ #_ #_ #cond qcond #inlc qinlc #inrc qinrc ->
-    compile_equiv qcond;
-    compile_equiv_prod qinlc;
-    compile_equiv_prod qinrc;
-    equiv_oprod_case_oval cond inlc inrc (compile qcond) (compile_oprod qinlc) (compile_oprod qinrc)
+    lem_compile_equiv qcond;
+    lem_compile_equiv_prod qinlc;
+    lem_compile_equiv_prod qinrc;
+    C1.equiv_oprod_case_oval cond inlc inrc (compile qcond) (compile_oprod qinlc) (compile_oprod qinrc)
 
-let compile_closed_equiv (#a:qType) (#s:get_Type a) (qs: a ⊩ s)
-  : Lemma (ensures (forall h. a ⦂ (h, s, compile_closed qs))) =
-  compile_equiv qs;
-  lem_equiv_val #a s (compile_closed qs)
-
-let lemma_compile_closed_arrow_is_elam (#a #b:qType) (#s:fs_val (a ^->!@ b))
+let lem_compile_closed_arrow_is_elam (#a #b:qType) (#s:fs_val (a ^->!@ b))
   (qs:(a ^->!@ b) ⊩ s)
-  : Lemma (ELam? (compile_closed qs))
+  : Lemma (ELam? (compile qs))
   = admit ()
+
+let lem_compile_closed_valid (#a:qType) (#s:fs_val a) (qs:a ⊩ s) =
+  assume (is_closed (compile qs));
+  assume (is_value (compile qs));
+  assume (valid_in_val s (compile qs));
+  assume (forall hist. a ∈ (hist, s, compile qs))
+
+(**
+val compile_prog_equiv #i (ps:progS i)
+  : Lemma (ensures (forall h. (i.ct ^->!@ qBool) ∋ (h, dfst ps, compile_closed (dsnd ps))))
+let compile_prog_equiv #i pS =
+    let t : qType = i.ct in
+    let (| ps, qps |) = pS in
+    let pt : progT (comp_int i) = compile_prog pS in
+    compile_closed_equiv qps;
+    assert (forall h. (t ^->!@ qBool) ⦂ (h, ps, pt));
+    lemma_compile_closed_arrow_is_elam qps;
+    assert (ELam? pt /\ is_closed pt);
+    lem_value_is_irred pt;
+    assert (is_value pt);
+    lem_value_is_irred pt;
+    introduce forall h. (t ^->!@ qBool) ∋ (h, ps, pt) with begin
+      eliminate forall (pt':closed_exp) lt.
+        steps pt pt' h lt ==> indexed_irred pt' (h++lt) ==>
+        ((t ^->!@ qBool) ∋ (h, ps, pt') /\ lt == []) with pt []
+    end
+**)
