rupicola/io/LogRelSourceTarget.CompatibilityLemmas.fst
@@ -1,304 +1,13 @@
-module ExpRel
+module LogRelSourceTarget.CompatibilityLemmas
 
-open FStar.Tactics
-open FStar.Classical.Sugar
-open FStar.List.Tot
-
+open Trace
 open STLC
 open QTyp
 open IO
-open Trace
+open LogRelSourceTarget
 
-(** Section 8.1: https://www.cs.uoregon.edu/research/summerschool/summer24/lectures/Ahmed.pdf **)
 
-let io_oexp (g:typ_env) (t:qType) =
-  eval_env g -> io (get_Type t)
-
-unfold val fs_beh : #t:qType -> fs_prod t -> h:history -> hist_post h (get_Type t)
-let fs_beh m = thetaP m
-
-unfold val e_beh : closed_exp -> closed_exp -> h:history -> local_trace h -> Type0
-let e_beh e e' h lt =
-  steps e e' h lt /\ indexed_irred e' (h++lt)
-
-(** Cross Language Binary Logical Relation between F* and STLC expressions
-     for __closed terms__. **)
-let rec (∋) (t:qType) (p:(history * fs_val t * closed_exp)) : Tot Type0 (decreases %[get_rel t;0]) =
-  let (h, fs_v, e) = p in
-  match get_rel t with // way to "match" on F* types
-  | QUnit -> fs_v == () /\ e == EUnit
-  | QBool -> (fs_v == true /\ e == ETrue) \/ (fs_v == false /\ e == EFalse)
-  | QFileDescriptor ->  e == EFileDescr fs_v
-  | QArr #t1 #t2 qt1 qt2 -> begin
-    let fs_f : t1 -> t2 = fs_v in
-    match e with
-    | ELam e' ->
-      (forall (v:value) (fs_v:t1) (lt_v:local_trace h). pack qt1 ∋ (h++lt_v, fs_v, v) ==>
-        pack qt2 ⦂ (h++lt_v, fs_f fs_v, subst_beta v e'))
-    | _ -> False
-  end
-  | QArrIO #t1 #t2 qt1 qt2 -> begin
-    let fs_f : t1 -> io t2 = fs_v in
-    match e with
-    | ELam e' -> // instead quantify over h'' - extensions of the history
-      (forall (v:value) (fs_v:t1) (lt_v:local_trace h). pack qt1 ∋ (h++lt_v, fs_v, v) ==>
-        pack qt2 ⪾ (h++lt_v, fs_f fs_v, subst_beta v e'))
-    | _ -> False
-  end
-  | QPair #t1 #t2 qt1 qt2 -> begin
-    match e with
-    | EPair e1 e2 -> (** e1 and e2 are values. no need to quantify over lts **)
-        pack qt1 ∋ (h, fst #t1 #t2 fs_v, e1) /\ pack qt2 ∋ (h, snd #t1 #t2 fs_v, e2)
-    | _ -> False
-  end
-  | QSum #t1 #t2 qt1 qt2 -> begin
-    let fs_v : either t1 t2 = fs_v in
-    match fs_v, e with
-    | Inl fs_v', EInl e' -> pack qt1 ∋ (h, fs_v', e')
-    | Inr fs_v', EInr e' -> pack qt2 ∋ (h, fs_v', e')
-    | _ -> False
-  end
-                           (** vvvvvvvvvv defined over values **)
-and (⦂) (t:qType) (p:history * fs_val t * closed_exp) : Tot Type0 (decreases %[get_rel t;1]) =
-  let (h, fs_e, e) = p in
-  forall (e':closed_exp) lt.
-    e_beh e e' h lt ==>
-    (t ∋ (h, fs_e, e') /\ lt == [])
-                           (** vvvvvvvvvv defined over producers **)
-and (⪾) (t:qType) (p:history * fs_prod t * closed_exp) : Tot Type0 (decreases %[get_rel t;1]) =
-  let (h, fs_e, e) = p in
-  forall lt.
-    (forall e'. e_beh e e' h lt ==>
-      (exists (fs_r:get_Type t). t ∋ (h++lt, fs_r, e') /\ fs_beh fs_e h lt fs_r))
-                           (** TODO: ^^^^^^^^^^^^^^^^^^^^^^^^^^^^^^^^^^ check this **)
-//    /\
-//    (forall (fs_r:get_Type t). fs_beh fs_e h lt fs_r ==>
-//      exists e'. t ∋ (h++lt, fs_r, e') /\ e_beh e e' h lt)
-
-let rec val_type_closed_under_history_extension (t:qType) (h:history) (fs_v:fs_val t) (e:closed_exp) :
-  Lemma (requires t ∋ (h, fs_v, e))
-        (ensures forall lt. t ∋ (h++lt, fs_v, e))
-        (decreases %[get_rel t;0]) =
-  introduce forall lt. t ∋ (h++lt, fs_v, e) with begin
-  match get_rel t with
-  | QUnit -> ()
-  | QBool -> ()
-  | QFileDescriptor -> ()
-  | QArr #t1 #t2 qt1 qt2 -> begin
-    let fs_f : t1 -> t2 = fs_v in
-    let ELam e' = e in
-    introduce forall (v:value) (fs_v':t1) (lt_v':local_trace (h++lt)). pack qt1 ∋ ((h++lt)++lt_v', fs_v', v) ==> pack qt2 ⦂ ((h++lt)++lt_v', fs_f fs_v', subst_beta v e') with begin
-      introduce pack qt1 ∋ ((h++lt)++lt_v', fs_v', v) ==> _ with _. begin
-        eliminate forall (v:value) (fs_v:t1) (lt_v:local_trace h). pack qt1 ∋ (h++lt_v, fs_v, v) ==> pack qt2 ⦂ (h++lt_v, fs_f fs_v, subst_beta v e') with v fs_v' (lt @ lt_v')
-      end
-    end
-    end
-  | QArrIO #t1 #t2 qt1 qt2 -> begin
-    let fs_f : t1 -> io t2 = fs_v in
-    let ELam e' = e in
-    introduce forall (v:value) (fs_v':t1) (lt_v':local_trace (h++lt)). pack qt1 ∋ ((h++lt)++lt_v', fs_v', v) ==> pack qt2 ⪾ ((h++lt)++lt_v', fs_f fs_v', subst_beta v e') with begin
-      introduce pack qt1 ∋ ((h++lt)++lt_v', fs_v', v) ==> _ with _. begin
-        eliminate forall (v:value) (fs_v:t1) (lt_v:local_trace h). pack qt1 ∋ (h++lt_v, fs_v, v) ==> pack qt2 ⪾ (h++lt_v, fs_f fs_v, subst_beta v e') with v fs_v' (lt @ lt_v')
-      end
-    end
-    end
-  | QPair #t1 #t2 qt1 qt2 -> begin
-    let EPair e1 e2 = e in
-    val_type_closed_under_history_extension (pack qt1) h (fst #t1 #t2 fs_v) e1;
-    val_type_closed_under_history_extension (pack qt2) h (snd #t1 #t2 fs_v) e2
-    end
-  | QSum #t1 #t2 qt1 qt2 -> begin
-    let fs_v : either t1 t2 = fs_v in
-    match fs_v, e with
-    | Inl fs_v', EInl e' -> val_type_closed_under_history_extension (pack qt1) h fs_v' e'
-    | Inr fs_v', EInr e' -> val_type_closed_under_history_extension (pack qt2) h fs_v' e'
-    | _ -> false_elim ()
-    end
-  end
-
-let lem_values_in_exp_rel_are_in_val_rel t fs_e (e:value) :
-  Lemma (requires forall h. t ⦂ (h, fs_e, e))
-        (ensures  forall h. t ∋ (h, fs_e, e)) = admit () (** TODO **)
-
-let lem_values_are_expressions t h fs_e e : (** lemma used by Amal **)
-  Lemma (requires t ∋ (h, fs_e, e))
-        (ensures  t ⦂ (h, fs_e, e)) = admit ()
-
-let lem_values_are_producers t h fs_e e : (** lemma used by Amal **)
-  Lemma (requires t ∋ (h, fs_e, e))
-        (ensures  t ⪾ (h, io_return fs_e, e)) = admit ()
-
-let rec lem_values_are_values t h fs_e (e:closed_exp) :
-  Lemma (requires t ∋ (h, fs_e, e))
-        (ensures is_value e)
-        (decreases e) =
-  match get_rel t with
-  | QUnit -> ()
-  | QBool -> ()
-  | QFileDescriptor -> ()
-  | QArr _ _ -> ()
-  | QArrIO _ _ -> ()
-  | QPair #t1 #t2 qt1 qt2 ->
-    let EPair e1 e2 = e in
-    lem_values_are_values (pack qt1) h (fst #t1 #t2 fs_e) e1;
-    lem_values_are_values (pack qt2) h (snd #t1 #t2 fs_e) e2
-  | QSum #t1 #t2 qt1 qt2 ->
-    match fs_e, e with
-    | Inl fs_e', EInl e' -> lem_values_are_values (pack qt1) h fs_e' e'
-    | Inr fs_e', EInr e' -> lem_values_are_values (pack qt2) h fs_e' e'
-
-let lem_forall_values_are_values t h fs_e :
-  Lemma (forall (e:closed_exp). t ∋ (h, fs_e, e) ==> is_value e) =
-  introduce forall e. t ∋ (h, fs_e, e) ==> is_value e with begin
-    introduce _ ==> _ with _. begin
-      lem_values_are_values t h fs_e e
-    end
-  end
-
-let lem_forall_values_are_values_prod t h :
-  Lemma (forall (e:closed_exp) (lt:local_trace h) (fs_r:get_Type t). t ∋ (h++lt, fs_r, e) ==> is_value e) =
-  introduce forall e lt fs_r. t ∋ (h++lt, fs_r, e) ==> is_value e with begin
-    introduce _ ==> _ with _. begin
-      lem_values_are_values t (h++lt) fs_r e
-    end
-  end
-
-(** F* Evaluation Environment : variable -> value **)
-
-(** We compile F* values, not F* expressions.
-    When compiling F* lambdas, there is no way to match and get
-    the body of the lambda.
-
-    To avoid this limitation, we do closure conversion of F* lambdas:
-    - be a lambda f:'a -> 'b
-    - we wrap f to a function that takes as argument an F* evaluation environment
-      that was extended to contain a value of type 'a
-    - we take the value from the environment to open f:
-        fun fsG -> f (index fsG 0)
-
-    What is cool about this is to define compilation to STLC the environment is abstract.
- **)
-
-let (∽) (#g:typ_env) #b (h:history) (fsG:eval_env g) (s:gsub g b) : Type0 =
-  forall (x:var). Some? (g x) ==>
-    Some?.v (g x) ∋ (h, index fsG x, s x)
-  (**  TODO      ^^^ not like in Amal's work. she uses an exp relation - but this is what she meant, because index fsG x is necessarily a value **)
-
-let lem_shift_type_value_environments (#g:typ_env) #b (h:history) (fsG:eval_env g) (s:gsub g b) :
-  Lemma (forall (lt:local_trace h). fsG `(∽) h` s ==> fsG `(∽) (h++lt)` s) =
-  introduce forall (lt:local_trace h). fsG `(∽) h` s ==> fsG `(∽) (h++lt)` s with begin
-    introduce _ ==> _ with _. begin
-      introduce forall (x:var). Some? (g x) ==> Some?.v (g x) ∋ (h++lt, index fsG x, s x) with begin
-        introduce _ ==> _ with _. begin
-          val_type_closed_under_history_extension (Some?.v (g x)) h (index fsG x) (s x)
-        end
-      end
-    end
-  end
-
-(** Cross Language Binary Logical Relation between F* and STLC expressions
-     for __open terms__. **)
-let equiv_oval (#g:typ_env) (t:qType) (fs_e:fs_oval g t) (e:exp) : Type0 =
-  fv_in_env g e /\
-  forall b (s:gsub g b) (fsG:eval_env g) (h:history).
-    fsG `(∽) h` s ==> t ⦂ (h, fs_e fsG, gsubst s e)
-
-let equiv_oprod (#g:typ_env) (t:qType) (fs_e:fs_oprod g t) (e:exp) : Type0 =
-  fv_in_env g e /\
-  forall b (s:gsub g b) (fsG:eval_env g) (h:history).
-    fsG `(∽) h` s ==> t ⪾ (h, fs_e fsG, gsubst s e)
-
-let equiv_val (#t:qType) (fs_e:fs_val t) (e:exp) : Type0 =
-  equiv_oval #empty t (fun _ -> fs_e) e
-
-let equiv_prod (#t:qType) (fs_e:fs_prod t) (e:exp) : Type0 =
-  equiv_oprod #empty t (fun _ -> fs_e) e
-
-let safety_val (#t:qType) (fs_e:fs_val t) (e:exp) : Lemma
-  (requires (equiv_val fs_e e))
-  (ensures forall h'. indexed_safe e h') =
-  admit ()
-
-let safety_prod (#t:qType) (fs_e:fs_prod t) (e:exp) : Lemma
-  (requires (equiv_prod fs_e e))
-  (ensures safe e) =
-  introduce forall (e':closed_exp) (h:history) (lt:local_trace h).
-    steps e e' h lt ==> is_value e' \/ indexed_can_step e' (h++lt) with begin
-    introduce steps e e' h lt ==> is_value e' \/ indexed_can_step e' (h++lt) with _. begin
-      introduce indexed_irred e' (h++lt) ==> is_value e' with _. begin
-        eliminate forall b (s:gsub empty b) (fsG:eval_env empty) (h:history).
-          fsG `(∽) h` s ==> t ⪾ (h, fs_e, gsubst s e)
-        with  true gsub_empty empty_eval h;
-        assert (t ⪾ (h, fs_e, e));
-        eliminate exists (fs_r:get_Type t). t ∋ (h++lt, fs_r, e') /\ fs_beh fs_e h lt fs_r
-        returns is_value e' with _. begin
-          assert (t ∋ (h++lt, fs_r, e'));
-          lem_values_are_values t (h++lt) fs_r e';
-          assert (is_value e')
-        end
-      end
-    end
-  end
-
-let sem_expr_shape_val (#t:qType) (fs_e:fs_val t) (e:exp) (h:history) :
-  Lemma (requires equiv_val fs_e e)
-        (ensures indexed_sem_expr_shape (type_quotation_to_typ (get_rel t)) e h) =  admit ()
-
-let sem_expr_shape_prod (#t:qType) (fs_e:fs_prod t) (e:exp) (h:history) :
-  Lemma (requires equiv_prod fs_e e)
-        (ensures indexed_sem_expr_shape (type_quotation_to_typ (get_rel t)) e h) =
-  introduce forall e' (lt:local_trace h). e_beh e e' h lt ==> sem_value_shape (type_quotation_to_typ (get_rel t)) e' with begin
-    introduce e_beh e e' h lt ==> sem_value_shape (type_quotation_to_typ (get_rel t)) e' with _. begin
-      eliminate forall b (s:gsub empty b) (fsG:eval_env empty) (h:history).
-          fsG `(∽) h` s ==> t ⪾ (h, fs_e, gsubst s e)
-      with  true gsub_empty empty_eval h;
-      assert (t ⪾ (h, fs_e, e));
-      eliminate exists (fs_r:get_Type t). t ∋ (h++lt, fs_r, e')
-      returns sem_value_shape (type_quotation_to_typ (get_rel t)) e' with _. begin
-      lem_values_are_values t (h++lt) fs_r e'
-      end
-    end
-  end
-
-let (≈) (#g:typ_env) (#t:qType) (fs_v:fs_oval g t) (e:exp) : Type0 =
-  equiv_oval #g t fs_v e
-
-let (≋) (#g:typ_env) (#t:qType) (fs_v:fs_oprod g t) (e:exp) : Type0 =
-  equiv_oprod #g t fs_v e
-
-(** Equiv closed terms **)
-let lem_equiv_val (#t:qType) (fs_e:fs_val t) (e:closed_exp) :
-  Lemma (requires equiv_val fs_e e)
-        (ensures forall h. t ⦂ (h, fs_e, e)) =
-  admit ()
-
-(**
-let lem_equiv_val' (#t:qType) (fs_e:fs_val t) (e:closed_exp) :
-  Lemma (requires forall h. t ⦂ (h, fs_e, e))
-        (ensures equiv_val fs_e e) =
-  admit ()
-**)
-
-let lem_equiv_prod (#t:qType) (fs_e:fs_prod t) (e:closed_exp) :
-  Lemma (requires equiv_prod fs_e e)
-        (ensures forall h. t ⪾ (h, fs_e, e)) =
-  eliminate forall b (s:gsub empty b) (fsG:eval_env empty). forall h.
-    fsG `(∽) h` s ==> t ⪾ (h, (fun _ -> fs_e) fsG, gsubst s e) with true gsub_empty empty_eval
-
-let lem_equiv_prod' (g:typ_env) (#t:qType) (fs_e:fs_prod t) (e:closed_exp) :
-  Lemma (requires (forall h. t ⪾ (h, fs_e, e)))
-        (ensures equiv_prod fs_e e) =
-  introduce forall b (s:gsub empty b) (fsG:eval_env empty) (h':history).
-    fsG `(∽) h'` s ==> t ⪾ (h', (fun _ -> fs_e) fsG, gsubst s e) with begin
-    introduce fsG `(∽) h'` s ==> t ⪾ (h', (fun _ -> fs_e) fsG, gsubst s e) with _. begin
-      assert (gsubst s e == e);
-      assert ((fun _ -> fs_e) fsG == fs_e);
-      eliminate forall h. t ⪾ (h, fs_e, e) with h'
-    end
-  end
-
-(** Rules **)
-let equiv_unit g : Lemma (fs_oval_return g qUnit () ≈ EUnit) =
+let equiv_oval_unit g : Lemma (fs_oval_return g qUnit () ≈ EUnit) =
   introduce forall b (s:gsub g b) fsG h. fsG `(∽) h` s ==> qUnit ⦂ (h, (), gsubst s EUnit) with begin
     introduce _ ==> _ with _. begin
       assert (qUnit ∋ (h, (), EUnit));
@@ -306,7 +15,7 @@ let equiv_unit g : Lemma (fs_oval_return g qUnit () ≈ EUnit) =
     end
   end
 
-let equiv_true g : Lemma (fs_oval_return g qBool true ≈ ETrue) =
+let equiv_oval_true g : Lemma (fs_oval_return g qBool true ≈ ETrue) =
   introduce forall b (s:gsub g b) fsG h. fsG `(∽) h` s ==> qBool ⦂ (h, true, gsubst s ETrue) with begin
     introduce _ ==> _ with _. begin
       assert (qBool ∋ (h, true, ETrue));
@@ -314,7 +23,7 @@ let equiv_true g : Lemma (fs_oval_return g qBool true ≈ ETrue) =
     end
   end
 
-let equiv_false g : Lemma (fs_oval_return g qBool false ≈ EFalse) =
+let equiv_oval_false g : Lemma (fs_oval_return g qBool false ≈ EFalse) =
   introduce forall b (s:gsub g b) fsG h. fsG `(∽) h` s ==> qBool ⦂ (h, false, gsubst s EFalse) with begin
     introduce _ ==> _ with _. begin
       assert (qBool ∋ (h, false, EFalse));
@@ -322,7 +31,7 @@ let equiv_false g : Lemma (fs_oval_return g qBool false ≈ EFalse) =
     end
   end
 
-let equiv_file_descr g fd : Lemma (fs_oval_return g qFileDescr fd ≈ EFileDescr fd) =
+let equiv_oval_file_descr g fd : Lemma (fs_oval_return g qFileDescr fd ≈ EFileDescr fd) =
   introduce forall b (s:gsub g b) fsG h. fsG `(∽) h` s ==> qFileDescr ⦂ (h, fd, gsubst s (EFileDescr fd)) with begin
     introduce _ ==> _ with _. begin
       assert (qFileDescr ∋ (h, fd, (EFileDescr fd)));
@@ -331,7 +40,7 @@ let equiv_file_descr g fd : Lemma (fs_oval_return g qFileDescr fd ≈ EFileDescr
   end
 
 (** Used in backtranslation **)
-let equiv_var g (x:var{Some? (g x)}) : Lemma (fs_oval_var g x ≈ EVar x) =
+let equiv_oval_var g (x:var{Some? (g x)}) : Lemma (fs_oval_var g x ≈ EVar x) =
   introduce forall b (s:gsub g b) fsG h. fsG `(∽) h` s ==> Some?.v (g x) ⦂ (h, index fsG x, gsubst s (EVar x)) with begin
     introduce _ ==> _ with _. begin
       assert (Some?.v (g x) ∋ (h, index fsG x, s x));
@@ -340,7 +49,7 @@ let equiv_var g (x:var{Some? (g x)}) : Lemma (fs_oval_var g x ≈ EVar x) =
   end
 
 (** Used in compilation **)
-let equiv_var0 (g:typ_env) (t:qType) : Lemma (fs_oval_var0 g t ≈ EVar 0) =
+let equiv_oval_var0 (g:typ_env) (t:qType) : Lemma (fs_oval_var0 g t ≈ EVar 0) =
   introduce forall b (s:gsub (extend t g) b) fsG h. fsG `(∽) h` s ==>  t ⦂ (h, hd fsG, gsubst s (EVar 0)) with begin
     introduce _ ==> _ with _. begin
       index_0_hd fsG;
@@ -468,7 +177,7 @@ let equiv_varS (#g:typ_env) #a #t (s:fs_oval g a) (e:exp)
   end
 #pop-options
 
-let equiv_lam #g (#t1:qType) (#t2:qType) (fs_body:fs_oval (extend t1 g) t2) (body:exp) : Lemma
+let equiv_oval_lambda #g (#t1:qType) (#t2:qType) (fs_body:fs_oval (extend t1 g) t2) (body:exp) : Lemma
   (requires fs_body ≈ body)
   (ensures (fs_oval_lambda fs_body ≈ ELam body)) =
   lem_fv_in_env_lam g t1 body;
@@ -507,30 +216,14 @@ let equiv_lam #g (#t1:qType) (#t2:qType) (fs_body:fs_oval (extend t1 g) t2) (bod
     end
   end
 
-let unroll_elam (t1 t2:qType) (h:history) (fs_e1:fs_val (t1 ^-> t2)) (e11:exp)
-  : Lemma (requires (is_closed (ELam e11)) /\ ((t1 ^-> t2) ∋ (h, fs_e1, ELam e11)))
-          (ensures (forall (v:value) (fs_v:fs_val t1) (lt_v:local_trace h). t1 ∋ (h++lt_v, fs_v, v) ==> t2 ⦂ (h++lt_v, fs_e1 fs_v, subst_beta v e11))) = admit ()
-
-let unroll_elam_io (t1 t2:qType) (h:history) (fs_e1:fs_val (t1 ^->!@ t2)) (e11:exp)
-  : Lemma (requires (is_closed (ELam e11)) /\ ((t1 ^->!@ t2) ∋ (h, fs_e1, ELam e11)))
-          (ensures (forall (v:value) (fs_v:fs_val t1) (lt_v:local_trace h). t1 ∋ (h++lt_v, fs_v, v) ==> t2 ⪾ (h++lt_v, fs_e1 fs_v, subst_beta v e11))) = admit ()
-
-let unroll_elam_io' (t1 t2:qType) (fs_e1:fs_val (t1 ^->!@ t2)) (e11:exp)
-  : Lemma (requires (is_closed (ELam e11)) /\ (forall h. (t1 ^->!@ t2) ∋ (h, fs_e1, ELam e11)))
-          (ensures (forall h (v:value) (fs_v:fs_val t1) (lt_v:local_trace h). t1 ∋ (h++lt_v, fs_v, v) ==> t2 ⪾ (h++lt_v, fs_e1 fs_v, subst_beta v e11))) =
-  introduce forall h. forall (v:value) (fs_v:fs_val t1) (lt_v:local_trace h). t1 ∋ (h++lt_v, fs_v, v) ==> t2 ⪾ (h++lt_v, fs_e1 fs_v, subst_beta v e11) with
-
-
-    unroll_elam_io t1 t2 h fs_e1 e11
-
-let equiv_app_steps_pre (e e':closed_exp) (h:history) (lt:local_trace h) (t1 t2:qType) (fs_e1:get_Type (t1 ^-> t2)) (fs_e2:get_Type t1) (fs_e:get_Type t2) (e1 e2:closed_exp) =
+let helper_equiv_oval_app_steps_pre (e e':closed_exp) (h:history) (lt:local_trace h) (t1 t2:qType) (fs_e1:get_Type (t1 ^-> t2)) (fs_e2:get_Type t1) (fs_e:get_Type t2) (e1 e2:closed_exp) =
   (fs_e == fs_e1 fs_e2) /\
   (e == EApp e1 e2) /\
   (e_beh e e' h lt) /\
   (t1 ⦂ (h, fs_e2, e2)) /\
   (forall (lt:local_trace h). (t1 ^-> t2) ⦂ (h++lt, fs_e1, e1))
 
-let equiv_app_steps #e #e' #h #lt #t1 #t2 #fs_e1 #fs_e2 #fs_e #e1 #e2 (sq:squash (equiv_app_steps_pre e e' h lt t1 t2 fs_e1 fs_e2 fs_e e1 e2)) : squash (t2 ∋ (h, fs_e, e') /\ lt == []) =
+let helper_equiv_oval_app_steps #e #e' #h #lt #t1 #t2 #fs_e1 #fs_e2 #fs_e #e1 #e2 (sq:squash (helper_equiv_oval_app_steps_pre e e' h lt t1 t2 fs_e1 fs_e2 fs_e e1 e2)) : squash (t2 ∋ (h, fs_e, e') /\ lt == []) =
   lem_forall_values_are_values t1 h fs_e2;
   assert (forall e2' lt2. e_beh e2 e2' h lt2 ==> is_value e2');
   FStar.Squash.bind_squash #(steps e e' h lt) () (fun steps_e_e' ->
@@ -548,7 +241,7 @@ let equiv_app_steps #e #e' #h #lt #t1 #t2 #fs_e1 #fs_e2 #fs_e #e1 #e2 (sq:squash
   assert (t2 ⦂ (h, fs_e, subst_beta e2' e11));
   assert (t2 ∋ (h, fs_e, e'))))
 
-let equiv_app #g
+let equiv_oval_app #g
   (#t1:qType) (#t2:qType)
   (fs_e1:fs_oval g (t1 ^-> t2)) (fs_e2:fs_oval g t1)
   (e1:exp) (e2:exp)
@@ -567,15 +260,15 @@ let equiv_app #g
       introduce forall (e':closed_exp) lt. e_beh e e' h lt ==> (t2 ∋ (h, fs_e, e') /\ lt == []) with begin
         introduce e_beh e e' h lt ==> (t2 ∋ (h, fs_e, e') /\ lt == []) with _. begin
           lem_shift_type_value_environments h fsG s;
-          let steps_pre : squash (equiv_app_steps_pre e e' h lt t1 t2 fs_e1 fs_e2 fs_e e1 e2) = () in
+          let steps_pre : squash (helper_equiv_oval_app_steps_pre e e' h lt t1 t2 fs_e1 fs_e2 fs_e e1 e2) = () in
           FStar.Squash.map_squash #_ #(squash (t2 ∋ (h, fs_e, e') /\ lt == [])) steps_pre (fun steps_pre ->
-          equiv_app_steps #e #e' #h #lt #t1 #t2 #fs_e1 #fs_e2 #fs_e #e1 #e2 steps_pre)
+          helper_equiv_oval_app_steps #e #e' #h #lt #t1 #t2 #fs_e1 #fs_e2 #fs_e #e1 #e2 steps_pre)
         end
       end
     end
   end
 
-let equiv_if_steps_pre (e e':closed_exp) (h:history) (lt:local_trace h) (t:qType) (fs_e1:bool) (fs_e2 fs_e3 fs_e:get_Type t) (e1:closed_exp) (e2:closed_exp) (e3:closed_exp) =
+let helper_equiv_oval_if_steps_pre (e e':closed_exp) (h:history) (lt:local_trace h) (t:qType) (fs_e1:bool) (fs_e2 fs_e3 fs_e:get_Type t) (e1:closed_exp) (e2:closed_exp) (e3:closed_exp) =
   (fs_e == (if fs_e1 then fs_e2 else fs_e3)) /\
   (e == (EIf e1 e2 e3)) /\
   (steps (EIf e1 e2 e3) e' h lt) /\
@@ -584,7 +277,7 @@ let equiv_if_steps_pre (e e':closed_exp) (h:history) (lt:local_trace h) (t:qType
   (t ⦂ (h, fs_e2, e2)) /\
   (t ⦂ (h, fs_e3, e3))
 
-let equiv_if_steps #e #e' #h #lt #t #fs_e1 #fs_e2 #fs_e3 #fs_e #e1 #e2 #e3 (sq:squash (equiv_if_steps_pre e e' h lt t fs_e1 fs_e2 fs_e3 fs_e e1 e2 e3)) : squash (t ∋ (h, fs_e, e') /\ lt == []) =
+let helper_equiv_oval_if_steps #e #e' #h #lt #t #fs_e1 #fs_e2 #fs_e3 #fs_e #e1 #e2 #e3 (sq:squash (helper_equiv_oval_if_steps_pre e e' h lt t fs_e1 fs_e2 fs_e3 fs_e e1 e2 e3)) : squash (t ∋ (h, fs_e, e') /\ lt == []) =
   assert (forall e1' lt1. e_beh e1 e1' h lt1 ==> (ETrue? e1' \/ EFalse? e1'));
   FStar.Squash.bind_squash #(steps e e' h lt) () (fun sts ->
   let (e1', (| lt1, (lt2, lt3) |)) = destruct_steps_eif e1 e2 e3 e' h lt sts in
@@ -596,7 +289,7 @@ let equiv_if_steps #e #e' #h #lt #t #fs_e1 #fs_e2 #fs_e3 #fs_e #e1 #e2 #e3 (sq:s
     assert (t ∋ (h, fs_e3, e') /\ lt3 == [])
   end)
 
-let equiv_if #g
+let equiv_oval_if #g
   (#t:qType)
   (fs_e1:fs_oval g qBool) (fs_e2:fs_oval g t) (fs_e3:fs_oval g t)
   (e1:exp) (e2:exp) (e3:exp)
@@ -615,22 +308,22 @@ let equiv_if #g
     introduce fsG `(∽) h` s ==> t ⦂ (h, fs_e, e) with _. begin
       introduce forall (e':closed_exp) lt. e_beh e e' h lt ==> (t ∋ (h, fs_e, e') /\ lt == []) with begin
         introduce e_beh e e' h lt ==> (t ∋ (h, fs_e, e') /\ lt == []) with _. begin
-          let steps_pre : squash (equiv_if_steps_pre e e' h lt t fs_e1 fs_e2 fs_e3 fs_e e1 e2 e3) = () in
+          let steps_pre : squash (helper_equiv_oval_if_steps_pre e e' h lt t fs_e1 fs_e2 fs_e3 fs_e e1 e2 e3) = () in
           FStar.Squash.map_squash #_ #(squash (t ∋ (h, fs_e, e') /\ lt == [])) steps_pre (fun steps_pre ->
-              equiv_if_steps #e #e' #h #lt #t #fs_e1 #fs_e2 #fs_e3 #fs_e #e1 #e2 #e3 steps_pre)
+              helper_equiv_oval_if_steps #e #e' #h #lt #t #fs_e1 #fs_e2 #fs_e3 #fs_e #e1 #e2 #e3 steps_pre)
         end
       end
     end
   end
 
-let equiv_pair_steps_pre (e e':closed_exp) (h:history) (lt:local_trace h) (t1 t2:qType) (fs_e1:get_Type t1) (fs_e2:get_Type t2) (fs_e:get_Type (t1 ^* t2)) (e1 e2:closed_exp) =
+let helper_equiv_oval_pair_steps_pre (e e':closed_exp) (h:history) (lt:local_trace h) (t1 t2:qType) (fs_e1:get_Type t1) (fs_e2:get_Type t2) (fs_e:get_Type (t1 ^* t2)) (e1 e2:closed_exp) =
   (fs_e == (fs_e1, fs_e2)) /\
   (e == EPair e1 e2) /\
   (e_beh e e' h lt) /\
   (t1 ⦂ (h, fs_e1, e1)) /\
   (forall (lt:local_trace h). t2 ⦂ (h++lt, fs_e2, e2))
 
-let equiv_pair_steps #e #e' #h #lt #t1 #t2 #fs_e1 #fs_e2 #fs_e #e1 #e2 (sq:squash (equiv_pair_steps_pre e e' h lt t1 t2 fs_e1 fs_e2 fs_e e1 e2)) : squash ((t1 ^* t2) ∋ (h, fs_e, e') /\ lt == []) =
+let helper_equiv_oval_pair_steps #e #e' #h #lt #t1 #t2 #fs_e1 #fs_e2 #fs_e #e1 #e2 (sq:squash (helper_equiv_oval_pair_steps_pre e e' h lt t1 t2 fs_e1 fs_e2 fs_e e1 e2)) : squash ((t1 ^* t2) ∋ (h, fs_e, e') /\ lt == []) =
   lem_forall_values_are_values t1 h fs_e1;
   assert (forall e1' lt1. e_beh e1 e1' h lt1 ==> is_value e1');
   FStar.Squash.bind_squash #(steps e e' h lt) () (fun steps_e_e' ->
@@ -646,7 +339,7 @@ let equiv_pair_steps #e #e' #h #lt #t1 #t2 #fs_e1 #fs_e2 #fs_e #e1 #e2 (sq:squas
   assert ((t1 ^* t2) ∋ (h, fs_e, EPair e1' e2'));
   lem_values_are_expressions (t1 ^* t2) h fs_e (EPair e1' e2')))
 
-let equiv_pair #g
+let equiv_oval_pair #g
   (#t1 #t2:qType)
   (fs_e1:fs_oval g t1) (fs_e2:fs_oval g t2)
   (e1:exp) (e2:exp)
@@ -666,21 +359,21 @@ let equiv_pair #g
       introduce forall (e':closed_exp) lt. e_beh e e' h lt ==> (t ∋ (h, fs_e, e') /\ lt == []) with begin
         introduce _ ==> (t ∋ (h, fs_e, e') /\ lt == []) with _. begin
           lem_shift_type_value_environments h fsG s;
-          let steps_pre : squash (equiv_pair_steps_pre e e' h lt t1 t2 fs_e1 fs_e2 fs_e e1 e2) = () in
+          let steps_pre : squash (helper_equiv_oval_pair_steps_pre e e' h lt t1 t2 fs_e1 fs_e2 fs_e e1 e2) = () in
           FStar.Squash.map_squash #_ #(squash ((t1 ^* t2) ∋ (h, fs_e, e') /\ lt == [])) steps_pre (fun steps_pre ->
-          equiv_pair_steps #e #e' #h #lt #t1 #t2 #fs_e1 #fs_e2 #fs_e #e1 #e2 steps_pre)
+          helper_equiv_oval_pair_steps #e #e' #h #lt #t1 #t2 #fs_e1 #fs_e2 #fs_e #e1 #e2 steps_pre)
         end
       end
     end
   end
 
-let equiv_pair_fst_steps_pre (e e':closed_exp) (h:history) (lt:local_trace h) (t1 t2:qType) (fs_e12:get_Type (t1 ^* t2)) (fs_e:get_Type t1) (e12:closed_exp) =
+let helper_equiv_oval_pair_fst_steps_pre (e e':closed_exp) (h:history) (lt:local_trace h) (t1 t2:qType) (fs_e12:get_Type (t1 ^* t2)) (fs_e:get_Type t1) (e12:closed_exp) =
   (fs_e == fst fs_e12) /\
   (e == EFst e12) /\
   (e_beh e e' h lt) /\
   ((t1 ^* t2) ⦂ (h, fs_e12, e12))
 
-let equiv_pair_fst_steps #e #e' #h #lt #t1 #t2 #fs_e12 #fs_e #e12 (sq:squash (equiv_pair_fst_steps_pre e e' h lt t1 t2 fs_e12 fs_e e12)) : squash (t1 ∋ (h, fs_e, e') /\ lt == []) =
+let helper_equiv_oval_pair_fst_steps #e #e' #h #lt #t1 #t2 #fs_e12 #fs_e #e12 (sq:squash (helper_equiv_oval_pair_fst_steps_pre e e' h lt t1 t2 fs_e12 fs_e e12)) : squash (t1 ∋ (h, fs_e, e') /\ lt == []) =
   lem_forall_values_are_values (t1 ^* t2) h fs_e12;
   assert (forall e12' lt12. e_beh e12 e12' h lt12 ==> (EPair? e12' /\ is_value e12'));
   FStar.Squash.bind_squash #(steps e e' h lt) () (fun steps_e_e' ->
@@ -699,7 +392,7 @@ let equiv_pair_fst_steps #e #e' #h #lt #t1 #t2 #fs_e12 #fs_e #e12 (sq:squash (eq
   assert (t1 ∋ (h, fs_e, e')))
 
 
-let equiv_pair_fst_app #g
+let equiv_oval_pair_fst_app #g
   (#t1 #t2:qType)
   (fs_e12:fs_oval g (t1 ^* t2))
   (e12:exp)
@@ -716,21 +409,21 @@ let equiv_pair_fst_app #g
     introduce fsG `(∽) h` s ==> t1 ⦂ (h, fs_e, e) with _. begin
       introduce forall (e':closed_exp) lt. e_beh e e' h lt ==> (t1 ∋ (h, fs_e, e') /\ lt == []) with begin
         introduce e_beh e e' h lt ==> (t1 ∋ (h, fs_e, e') /\ lt == []) with _. begin
-          let steps_pre : squash (equiv_pair_fst_steps_pre e e' h lt t1 t2 fs_e12 fs_e e12) = () in
+          let steps_pre : squash (helper_equiv_oval_pair_fst_steps_pre e e' h lt t1 t2 fs_e12 fs_e e12) = () in
           FStar.Squash.map_squash #_ #(squash (t1 ∋ (h, fs_e, e') /\ lt == [])) steps_pre (fun steps_pre ->
-          equiv_pair_fst_steps #e #e' #h #lt #t1 #t2 #fs_e12 #fs_e #e12 steps_pre)
+          helper_equiv_oval_pair_fst_steps #e #e' #h #lt #t1 #t2 #fs_e12 #fs_e #e12 steps_pre)
         end
       end
     end
   end
 
-let equiv_pair_snd_steps_pre (e e':closed_exp) (h:history) (lt:local_trace h) (t1 t2:qType) (fs_e12:get_Type (t1 ^* t2)) (fs_e:get_Type t2) (e12:closed_exp) =
+let helper_equiv_oval_pair_snd_steps_pre (e e':closed_exp) (h:history) (lt:local_trace h) (t1 t2:qType) (fs_e12:get_Type (t1 ^* t2)) (fs_e:get_Type t2) (e12:closed_exp) =
   (fs_e == snd fs_e12) /\
   (e == ESnd e12) /\
   (e_beh e e' h lt) /\
   ((t1 ^* t2) ⦂ (h, fs_e12, e12))
 
-let equiv_pair_snd_steps #e #e' #h #lt #t1 #t2 #fs_e12 #fs_e #e12 (sq:squash (equiv_pair_snd_steps_pre e e' h lt t1 t2 fs_e12 fs_e e12)) : squash (t2 ∋ (h, fs_e, e') /\ lt == []) =
+let helper_equiv_oval_pair_snd_steps #e #e' #h #lt #t1 #t2 #fs_e12 #fs_e #e12 (sq:squash (helper_equiv_oval_pair_snd_steps_pre e e' h lt t1 t2 fs_e12 fs_e e12)) : squash (t2 ∋ (h, fs_e, e') /\ lt == []) =
   lem_forall_values_are_values (t1 ^* t2) h fs_e12;
   assert (forall e12' lt12. e_beh e12 e12' h lt12 ==> (EPair? e12' /\ is_value e12'));
   FStar.Squash.bind_squash #(steps e e' h lt) () (fun steps_e_e' ->
@@ -748,9 +441,9 @@ let equiv_pair_snd_steps #e #e' #h #lt #t1 #t2 #fs_e12 #fs_e #e12 (sq:squash (eq
   lem_destruct_steps_epair_snd e1' e2' e' h lt_f;
   assert (t2 ∋ (h, fs_e, e')))
 
-let equiv_pair_snd_app #g (#t1 #t2:qType) (fs_e12:fs_oval g (t1 ^* t2)) (e12:exp)
+let equiv_oval_pair_snd_app #g (#t1 #t2:qType) (fs_e12:fs_oval g (t1 ^* t2)) (e12:exp)
   : Lemma
-    (requires fs_e12 ≈ e12) (** is this too strict? we only care for the left to be equivalent. **)
+    (requires fs_e12 ≈ e12)
     (ensures fs_oval_fmap fs_e12 snd ≈ (ESnd e12)) =
   lem_fv_in_env_snd g e12;
   introduce forall b (s:gsub g b) fsG h. fsG `(∽) h` s ==> t2 ⦂ (h, snd (fs_e12 fsG), gsubst s (ESnd e12)) with begin
@@ -762,21 +455,21 @@ let equiv_pair_snd_app #g (#t1 #t2:qType) (fs_e12:fs_oval g (t1 ^* t2)) (e12:exp
     introduce fsG `(∽) h` s ==> t2 ⦂ (h, fs_e, e) with _. begin
       introduce forall (e':closed_exp) lt. e_beh e e' h lt ==> (t2 ∋ (h, fs_e, e') /\ lt == []) with begin
         introduce e_beh e e' h lt ==> (t2 ∋ (h, fs_e, e') /\ lt == []) with _. begin
-        let steps_pre : squash (equiv_pair_snd_steps_pre e e' h lt t1 t2 fs_e12 fs_e e12) = () in
+        let steps_pre : squash (helper_equiv_oval_pair_snd_steps_pre e e' h lt t1 t2 fs_e12 fs_e e12) = () in
         FStar.Squash.map_squash #_ #(squash (t2 ∋ (h, fs_e, e') /\ lt == [])) steps_pre (fun steps_pre ->
-        equiv_pair_snd_steps #e #e' #h #lt #t1 #t2 #fs_e12 #fs_e #e12 steps_pre)
+        helper_equiv_oval_pair_snd_steps #e #e' #h #lt #t1 #t2 #fs_e12 #fs_e #e12 steps_pre)
         end
       end
     end
   end
 
-let equiv_inl_steps_pre (ex ex':closed_exp) (h:history) (lt:local_trace h) (t1 t2:qType) (fs_e:get_Type t1) (fs_ex:get_Type (t1 ^+ t2)) (e:closed_exp) =
+let helper_equiv_oval_inl_steps_pre (ex ex':closed_exp) (h:history) (lt:local_trace h) (t1 t2:qType) (fs_e:get_Type t1) (fs_ex:get_Type (t1 ^+ t2)) (e:closed_exp) =
   (fs_ex == Inl #(get_Type t1) #(get_Type t2) fs_e) /\
   (ex == EInl e) /\
   (e_beh ex ex' h lt) /\
   (t1 ⦂ (h, fs_e, e))
 
-let equiv_inl_steps #ex #ex' #h #lt #t1 #t2 #fs_e #fs_ex #e (sq:squash (equiv_inl_steps_pre ex ex' h lt t1 t2 fs_e fs_ex e)) : squash ((t1 ^+ t2) ∋ (h, fs_ex, ex') /\ lt == []) =
+let helper_equiv_oval_inl_steps #ex #ex' #h #lt #t1 #t2 #fs_e #fs_ex #e (sq:squash (helper_equiv_oval_inl_steps_pre ex ex' h lt t1 t2 fs_e fs_ex e)) : squash ((t1 ^+ t2) ∋ (h, fs_ex, ex') /\ lt == []) =
   lem_forall_values_are_values t1 h fs_e;
   assert (forall e' lt'. e_beh e e' h lt' ==> is_value e');
   FStar.Squash.bind_squash #(steps ex ex' h lt) () (fun steps_e_e' ->
@@ -787,7 +480,7 @@ let equiv_inl_steps #ex #ex' #h #lt #t1 #t2 #fs_e #fs_ex #e (sq:squash (equiv_in
   lem_destruct_steps_einl e' ex' h lt_f;
   assert ((t1 ^+ t2) ∋ (h, fs_ex, ex')))
 
-let equiv_inl #g (#t1 t2:qType) (fs_e:fs_oval g t1) (e:exp) : Lemma
+let equiv_oval_inl #g (#t1 t2:qType) (fs_e:fs_oval g t1) (e:exp) : Lemma
   (requires fs_e ≈ e)
   (ensures fs_oval_fmap #g #t1 #(t1 ^+ t2) fs_e Inl ≈ (EInl e)) =
   lem_fv_in_env_inl g e;
@@ -801,21 +494,21 @@ let equiv_inl #g (#t1 t2:qType) (fs_e:fs_oval g t1) (e:exp) : Lemma
     introduce fsG `(∽) h` s ==> t ⦂ (h, fs_ex, ex) with _. begin
       introduce forall (ex':closed_exp) lt. e_beh ex ex' h lt ==> (t ∋ (h, fs_ex, ex') /\ lt == []) with begin
         introduce _ ==> (t ∋ (h, fs_ex, ex') /\ lt == []) with _. begin
-        let steps_pre : squash (equiv_inl_steps_pre ex ex' h lt t1 t2 fs_e fs_ex e) = () in
+        let steps_pre : squash (helper_equiv_oval_inl_steps_pre ex ex' h lt t1 t2 fs_e fs_ex e) = () in
         FStar.Squash.map_squash #_ #(squash (t ∋ (h, fs_ex, ex') /\ lt == [])) steps_pre (fun steps_pre ->
-        equiv_inl_steps #ex #ex' #h #lt #t1 #t2 #fs_e #fs_ex #e steps_pre)
+        helper_equiv_oval_inl_steps #ex #ex' #h #lt #t1 #t2 #fs_e #fs_ex #e steps_pre)
         end
       end
     end
   end
 
-let equiv_inr_steps_pre (ex ex':closed_exp) (h:history) (lt:local_trace h) (t1 t2:qType) (fs_e:get_Type t2) (fs_ex:get_Type (t1 ^+ t2)) (e:closed_exp) =
+let helper_equiv_oval_inr_steps_pre (ex ex':closed_exp) (h:history) (lt:local_trace h) (t1 t2:qType) (fs_e:get_Type t2) (fs_ex:get_Type (t1 ^+ t2)) (e:closed_exp) =
   (fs_ex == Inr #(get_Type t1) #(get_Type t2) fs_e) /\
   (ex == EInr e) /\
   (e_beh ex ex' h lt) /\
   (t2 ⦂ (h, fs_e, e))
 
-let equiv_inr_steps #ex #ex' #h #lt #t1 #t2 #fs_e #fs_ex #e (sq:squash (equiv_inr_steps_pre ex ex' h lt t1 t2 fs_e fs_ex e)) : squash ((t1 ^+ t2) ∋ (h, fs_ex, ex') /\ lt == []) =
+let helper_equiv_oval_inr_steps #ex #ex' #h #lt #t1 #t2 #fs_e #fs_ex #e (sq:squash (helper_equiv_oval_inr_steps_pre ex ex' h lt t1 t2 fs_e fs_ex e)) : squash ((t1 ^+ t2) ∋ (h, fs_ex, ex') /\ lt == []) =
   lem_forall_values_are_values t2 h fs_e;
   assert (forall e' lt'. e_beh e e' h lt' ==> is_value e');
   FStar.Squash.bind_squash #(steps ex ex' h lt) () (fun steps_e_e' ->
@@ -826,7 +519,7 @@ let equiv_inr_steps #ex #ex' #h #lt #t1 #t2 #fs_e #fs_ex #e (sq:squash (equiv_in
   lem_destruct_steps_einr e' ex' h lt_f;
   assert ((t1 ^+ t2) ∋ (h, fs_ex, ex')))
 
-let equiv_inr #g (t1 #t2:qType) (fs_e:fs_oval g t2) (e:exp) : Lemma
+let equiv_oval_inr #g (t1 #t2:qType) (fs_e:fs_oval g t2) (e:exp) : Lemma
   (requires fs_e ≈ e)
   (ensures fs_oval_fmap #g #t2 #(t1 ^+ t2) fs_e Inr ≈ (EInr e)) =
   lem_fv_in_env_inr g e;
@@ -840,15 +533,15 @@ let equiv_inr #g (t1 #t2:qType) (fs_e:fs_oval g t2) (e:exp) : Lemma
     introduce fsG `(∽) h` s ==> t ⦂ (h, fs_ex, ex) with _. begin
       introduce forall (ex':closed_exp) lt. e_beh ex ex' h lt ==> (t ∋ (h, fs_ex, ex') /\ lt == []) with begin
         introduce _ ==> (t ∋ (h, fs_ex, ex') /\ lt == []) with _. begin
-        let steps_pre : squash (equiv_inr_steps_pre ex ex' h lt t1 t2 fs_e fs_ex e) = () in
+        let steps_pre : squash (helper_equiv_oval_inr_steps_pre ex ex' h lt t1 t2 fs_e fs_ex e) = () in
         FStar.Squash.map_squash #_ #(squash (t ∋ (h, fs_ex, ex') /\ lt == [])) steps_pre (fun steps_pre ->
-        equiv_inr_steps #ex #ex' #h #lt #t1 #t2 #fs_e #fs_ex #e steps_pre)
+        helper_equiv_oval_inr_steps #ex #ex' #h #lt #t1 #t2 #fs_e #fs_ex #e steps_pre)
         end
       end
     end
   end
 
-let equiv_case_steps_pre (e e':closed_exp) (h:history) (lt:local_trace h) (t1 t2 t3:qType) (fs_case:get_Type (t1 ^+ t2)) (fs_lc_lam:get_Type (t1 ^-> t3)) (fs_rc_lam:get_Type (t2 ^-> t3)) (fs_e:get_Type t3) (e_case:closed_exp) (e_lc:exp{is_closed (ELam e_lc)}) (e_rc:exp{is_closed (ELam e_rc)}) =
+let helper_equiv_oval_case_steps_pre (e e':closed_exp) (h:history) (lt:local_trace h) (t1 t2 t3:qType) (fs_case:get_Type (t1 ^+ t2)) (fs_lc_lam:get_Type (t1 ^-> t3)) (fs_rc_lam:get_Type (t2 ^-> t3)) (fs_e:get_Type t3) (e_case:closed_exp) (e_lc:exp{is_closed (ELam e_lc)}) (e_rc:exp{is_closed (ELam e_rc)}) =
   (fs_e == (match fs_case with
            | Inl x -> fs_lc_lam x
            | Inr x -> fs_rc_lam x)) /\
@@ -859,7 +552,7 @@ let equiv_case_steps_pre (e e':closed_exp) (h:history) (lt:local_trace h) (t1 t2
   ((t1 ^-> t3) ⦂ (h, fs_lc_lam, ELam e_lc)) /\
   ((t2 ^-> t3) ⦂ (h, fs_rc_lam, ELam e_rc))
 
-let equiv_case_steps #e #e' #h #lt #t1 #t2 #t3 #fs_case #fs_lc_lam #fs_rc_lam #fs_e #e_case #e_lc #e_rc (sq:squash (equiv_case_steps_pre e e' h lt t1 t2 t3 fs_case fs_lc_lam fs_rc_lam fs_e e_case e_lc e_rc)) : squash (t3 ∋ (h, fs_e, e') /\ lt == []) =
+let helper_equiv_oval_case_steps #e #e' #h #lt #t1 #t2 #t3 #fs_case #fs_lc_lam #fs_rc_lam #fs_e #e_case #e_lc #e_rc (sq:squash (helper_equiv_oval_case_steps_pre e e' h lt t1 t2 t3 fs_case fs_lc_lam fs_rc_lam fs_e e_case e_lc e_rc)) : squash (t3 ∋ (h, fs_e, e') /\ lt == []) =
   lem_forall_values_are_values (t1 ^+ t2) h fs_case;
   assert (forall e_case' lt'. e_beh e_case e_case' h lt' ==> ((EInl? e_case' \/ EInr? e_case') /\ is_value e_case'));
   FStar.Squash.bind_squash #(steps e e' h lt) () (fun sts ->
@@ -886,7 +579,7 @@ let equiv_case_steps #e #e' #h #lt #t1 #t2 #t3 #fs_case #fs_lc_lam #fs_rc_lam #f
     | _ -> false_elim ())
 
 #push-options "--z3rlimit 10000"
-let equiv_case
+let equiv_oval_case
   #g
   (#t1 #t2 #t3:qType)
   (fs_case:fs_oval g (t1 ^+ t2))
@@ -899,8 +592,8 @@ let equiv_case
   lem_fv_in_env_case g t1 t2 e_case e_lc e_rc;
   lem_fv_in_env_lam g t1 e_lc;
   lem_fv_in_env_lam g t2 e_rc;
-  equiv_lam #g #t1 #t3 fs_lc e_lc;
-  equiv_lam #g #t2 #t3 fs_rc e_rc;
+  equiv_oval_lambda #g #t1 #t3 fs_lc e_lc;
+  equiv_oval_lambda #g #t2 #t3 fs_rc e_rc;
   introduce forall b (s:gsub g b) fsG h. fsG `(∽) h` s ==> t3 ⦂ (h,
     (match fs_case fsG with
     | Inl x -> fs_lc (stack fsG x)
@@ -926,16 +619,16 @@ let equiv_case
         introduce e_beh e e' h lt ==> (t3 ∋ (h, fs_e, e') /\ lt == []) with _. begin
           assert ((t1 ^-> t3) ⦂ (h, fs_lc_lam, ELam e_lc));
           assert ((t2 ^-> t3) ⦂ (h, fs_rc_lam, ELam e_rc));
-          let steps_pre : squash (equiv_case_steps_pre e e' h lt t1 t2 t3 fs_case fs_lc_lam fs_rc_lam fs_e e_case e_lc e_rc) = () in
+          let steps_pre : squash (helper_equiv_oval_case_steps_pre e e' h lt t1 t2 t3 fs_case fs_lc_lam fs_rc_lam fs_e e_case e_lc e_rc) = () in
           FStar.Squash.map_squash #_ #(squash (t3 ∋ (h, fs_e, e') /\ lt == [])) steps_pre (fun steps_pre ->
-            equiv_case_steps #e #e' #h #lt #t1 #t2 #t3 #fs_case #fs_lc_lam #fs_rc_lam #fs_e #e_case #e_lc #e_rc steps_pre)
+            helper_equiv_oval_case_steps #e #e' #h #lt #t1 #t2 #t3 #fs_case #fs_lc_lam #fs_rc_lam #fs_e #e_case #e_lc #e_rc steps_pre)
         end
       end
     end
   end
 #pop-options
 
-let equiv_lam_prod #g (#t1:qType) (#t2:qType) (fs_body:fs_oprod (extend t1 g) t2) (body:exp)
+let equiv_oval_lambda_oprod #g (#t1:qType) (#t2:qType) (fs_body:fs_oprod (extend t1 g) t2) (body:exp)
   : Lemma
     (requires fs_body ≋ body)
     (ensures fs_oval_lambda_oprod fs_body ≈ (ELam body)) =
@@ -995,14 +688,14 @@ let equiv_oprod_return #g (#t:qType) (fs_x:fs_oval g t) (x:exp)
     end
   end
 
-let equiv_bind_steps_pre (e e':closed_exp) (h:history) (lt:local_trace h) (a:qType) (b:qType) (fs_k':(get_Type a) -> io (get_Type b)) (fs_m:io (get_Type a)) (fs_e':io (get_Type b)) (m:closed_exp) (k':exp) =
+let helper_equiv_oprod_bind_steps_pre (e e':closed_exp) (h:history) (lt:local_trace h) (a:qType) (b:qType) (fs_k':(get_Type a) -> io (get_Type b)) (fs_m:io (get_Type a)) (fs_e':io (get_Type b)) (m:closed_exp) (k':exp) =
   (fs_e' == io_bind fs_m fs_k') /\
   (e == EApp (ELam k') m) /\
   (e_beh e e' h lt) /\
   (a ⪾ (h, fs_m, m)) /\
   (forall (lt:local_trace h). ((a ^->!@ b) ⦂ (h++lt, fs_k', (ELam k'))))
 
-let equiv_bind_steps #e #e' #h #lt #a #b #fs_k' #fs_m #fs_e' #m #k' (sq:squash (equiv_bind_steps_pre e e' h lt a b fs_k' fs_m fs_e' m k')) : squash (exists (fs_r:get_Type b). b ∋ (h++lt, fs_r, e') /\ fs_beh fs_e' h lt fs_r) =
+let helper_equiv_oprod_bind_steps #e #e' #h #lt #a #b #fs_k' #fs_m #fs_e' #m #k' (sq:squash (helper_equiv_oprod_bind_steps_pre e e' h lt a b fs_k' fs_m fs_e' m k')) : squash (exists (fs_r:get_Type b). b ∋ (h++lt, fs_r, e') /\ fs_beh fs_e' h lt fs_r) =
   lem_forall_values_are_values_prod a h;
   assert (forall m' lt2. e_beh m m' h lt2 ==> is_value m');
   FStar.Squash.bind_squash #(steps e e' h lt) () (fun sts ->
@@ -1032,7 +725,7 @@ let equiv_oprod_bind #g (#a #b:qType) (fs_m:fs_oprod g a) (fs_k:fs_oprod (extend
     (ensures (fs_oprod_bind fs_m fs_k) ≋ (EApp (ELam k) m)) =
   lem_fv_in_env_lam g a k;
   lem_fv_in_env_app g (ELam k) m;
-  equiv_lam_prod fs_k k;
+  equiv_oval_lambda_oprod fs_k k;
   let fs_k' : fs_oval g (a ^->!@ b) = fun fsG x -> fs_k (stack fsG x) in
   introduce forall b' (s:gsub g b') fsG h. fsG `(∽) h` s ==> b ⪾ (h, io_bind (fs_m fsG) (fun x -> fs_k (stack fsG x)), gsubst s (EApp (ELam k) m)) with begin
     let fs_m = fs_m fsG in
@@ -1049,22 +742,22 @@ let equiv_oprod_bind #g (#a #b:qType) (fs_m:fs_oprod g a) (fs_k:fs_oprod (extend
       introduce forall lt (e':closed_exp). e_beh e e' h lt ==> (exists (fs_r:get_Type b). b ∋ (h++lt, fs_r, e') /\ fs_beh fs_e h lt fs_r) with begin
         introduce e_beh e e' h lt ==> (exists (fs_r:get_Type b). b ∋ (h++lt, fs_r, e') /\ fs_beh fs_e' h lt fs_r) with _. begin
           lem_shift_type_value_environments h fsG s;
-          let steps_pre : squash (equiv_bind_steps_pre e e' h lt a b fs_k' fs_m fs_e' m k') = () in
+          let steps_pre : squash (helper_equiv_oprod_bind_steps_pre e e' h lt a b fs_k' fs_m fs_e' m k') = () in
           FStar.Squash.map_squash #_ #(squash (exists (fs_r:get_Type b). b ∋ (h++lt, fs_r, e') /\ fs_beh fs_e' h lt fs_r)) steps_pre (fun steps_pre ->
-            equiv_bind_steps #e #e' #h #lt #a #b #fs_k' #fs_m #fs_e' #m #k' steps_pre)
+            helper_equiv_oprod_bind_steps #e #e' #h #lt #a #b #fs_k' #fs_m #fs_e' #m #k' steps_pre)
         end
       end
     end
   end
 
-let equiv_oprod_app_steps_pre (e e':closed_exp) (h:history) (lt:local_trace h) (a b:qType) (fs_f:get_Type (a ^->!@ b)) (fs_x:get_Type a) (fs_e:io (get_Type b)) (f x:closed_exp) =
+let helper_equiv_oprod_app_oval_oval_steps_pre (e e':closed_exp) (h:history) (lt:local_trace h) (a b:qType) (fs_f:get_Type (a ^->!@ b)) (fs_x:get_Type a) (fs_e:io (get_Type b)) (f x:closed_exp) =
   (fs_e == fs_f fs_x) /\
   (e == EApp f x) /\
   (e_beh e e' h lt) /\
   (a ⦂ (h, fs_x, x)) /\
   (forall (lt:local_trace h). (a ^->!@ b) ⦂ (h++lt, fs_f, f))
 
-let equiv_oprod_app_steps #e #e' #h #lt #a #b #fs_f #fs_x #fs_e #f #x (sq:squash (equiv_oprod_app_steps_pre e e' h lt a b fs_f fs_x fs_e f x)) : squash (exists (fs_r:get_Type b). b ∋ (h++lt, fs_r, e') /\ fs_beh fs_e h lt fs_r) =
+let helper_equiv_oprod_app_oval_oval_steps #e #e' #h #lt #a #b #fs_f #fs_x #fs_e #f #x (sq:squash (helper_equiv_oprod_app_oval_oval_steps_pre e e' h lt a b fs_f fs_x fs_e f x)) : squash (exists (fs_r:get_Type b). b ∋ (h++lt, fs_r, e') /\ fs_beh fs_e h lt fs_r) =
   lem_forall_values_are_values a h fs_x;
   FStar.Squash.bind_squash #(steps e e' h lt) () (fun steps_e_e' ->
   let (x', (| lt2, lt' |)) = destruct_steps_eapp_e2 f x e' h lt steps_e_e' in
@@ -1097,15 +790,15 @@ let equiv_oprod_app_oval_oval #g (#a #b:qType) (fs_f:fs_oval g (a ^->!@ b)) (fs_
       introduce forall lt (e':closed_exp). e_beh e e' h lt ==> (exists (fs_r:get_Type b). b  ∋ (h++lt, fs_r, e') /\ (fs_beh fs_e h lt fs_r)) with begin
         introduce _ ==> (exists (fs_r:get_Type b). b ∋ (h++lt, fs_r, e') /\ fs_beh fs_e h lt fs_r) with _. begin
         lem_shift_type_value_environments h fsG s;
-        let steps_pre : squash (equiv_oprod_app_steps_pre e e' h lt a b fs_f fs_x fs_e f x) = () in
+        let steps_pre : squash (helper_equiv_oprod_app_oval_oval_steps_pre e e' h lt a b fs_f fs_x fs_e f x) = () in
         FStar.Squash.map_squash #_ #(squash (exists (fs_r:get_Type b). b ∋ (h++lt, fs_r, e') /\ fs_beh fs_e h lt fs_r)) steps_pre (fun steps_pre ->
-        equiv_oprod_app_steps #e #e' #h #lt #a #b #fs_f #fs_x #fs_e #f #x steps_pre)
+        helper_equiv_oprod_app_oval_oval_steps #e #e' #h #lt #a #b #fs_f #fs_x #fs_e #f #x steps_pre)
         end
       end
     end
   end
 
-let equiv_if_prod_steps_pre (ex ex':closed_exp) (h:history) (lt:local_trace h) (a:qType) (fs_c:bool) (fs_t fs_e fs_ex:fs_prod a) (c t e:closed_exp) =
+let helper_equiv_oprod_if_oval_steps_pre (ex ex':closed_exp) (h:history) (lt:local_trace h) (a:qType) (fs_c:bool) (fs_t fs_e fs_ex:fs_prod a) (c t e:closed_exp) =
   (fs_ex == (if fs_c then fs_t else fs_e)) /\
   (ex == (EIf c t e)) /\
   (e_beh ex ex' h lt) /\
@@ -1113,7 +806,7 @@ let equiv_if_prod_steps_pre (ex ex':closed_exp) (h:history) (lt:local_trace h) (
   (a ⪾ (h, fs_t, t)) /\
   (a ⪾ (h, fs_e, e))
 
-let equiv_if_prod_steps #ex #ex' #h #lt #a #fs_c #fs_t #fs_e #fs_ex #c #t #e (sq:squash (equiv_if_prod_steps_pre ex ex' h lt a fs_c fs_t fs_e fs_ex c t e)) : squash (exists (fs_r:get_Type a). a ∋ (h++lt, fs_r, ex') /\ fs_beh fs_ex h lt fs_r) =
+let helper_equiv_oprod_if_oval_steps #ex #ex' #h #lt #a #fs_c #fs_t #fs_e #fs_ex #c #t #e (sq:squash (helper_equiv_oprod_if_oval_steps_pre ex ex' h lt a fs_c fs_t fs_e fs_ex c t e)) : squash (exists (fs_r:get_Type a). a ∋ (h++lt, fs_r, ex') /\ fs_beh fs_ex h lt fs_r) =
   assert (forall c' lt'. e_beh c c' h lt' ==> (ETrue? c' \/ EFalse? c'));
   FStar.Squash.bind_squash #(steps ex ex' h lt) () (fun sts ->
   let (c', (| lt1, (lt2, lt3) |)) = destruct_steps_eif c t e ex' h lt sts in
@@ -1141,15 +834,15 @@ let equiv_oprod_if_oval #g (#a:qType) (fs_c:fs_oval g qBool) (fs_t fs_e:fs_oprod
     introduce fsG `(∽) h` s ==> a ⪾ (h, fs_ex, ex) with _. begin
       introduce forall lt (ex':closed_exp). e_beh ex ex' h lt ==> (exists (fs_r:get_Type a). a ∋ (h++lt, fs_r, ex') /\ fs_beh fs_ex h lt fs_r) with begin
         introduce e_beh ex ex' h lt ==> (exists (fs_r:get_Type a). a ∋ (h++lt, fs_r, ex') /\ fs_beh fs_ex h lt fs_r) with _. begin
-          let steps_pre : squash (equiv_if_prod_steps_pre ex ex' h lt a fs_c fs_t fs_e fs_ex c t e) = () in
+          let steps_pre : squash (helper_equiv_oprod_if_oval_steps_pre ex ex' h lt a fs_c fs_t fs_e fs_ex c t e) = () in
           FStar.Squash.map_squash #_ #(squash (exists (fs_r:get_Type a). a ∋ (h++lt, fs_r, ex') /\ fs_beh fs_ex h lt fs_r)) steps_pre (fun steps_pre ->
-            equiv_if_prod_steps #ex #ex' #h #lt #a #fs_c #fs_t #fs_e #fs_ex #c #t #e steps_pre)
+            helper_equiv_oprod_if_oval_steps #ex #ex' #h #lt #a #fs_c #fs_t #fs_e #fs_ex #c #t #e steps_pre)
         end
       end
     end
   end
 
-let equiv_case_prod_steps_pre (e e':closed_exp) (h:history) (lt:local_trace h) (a b c:qType) (fs_cond:get_Type (a ^+ b)) (fs_inlc:get_Type (a ^->!@ c)) (fs_inrc:get_Type (b ^->!@ c)) (fs_e:fs_prod c) (cond:closed_exp) (inlc:exp{is_closed (ELam inlc)}) (inrc:exp{is_closed (ELam inrc)}) =
+let helper_equiv_oprod_case_oval_steps_pre (e e':closed_exp) (h:history) (lt:local_trace h) (a b c:qType) (fs_cond:get_Type (a ^+ b)) (fs_inlc:get_Type (a ^->!@ c)) (fs_inrc:get_Type (b ^->!@ c)) (fs_e:fs_prod c) (cond:closed_exp) (inlc:exp{is_closed (ELam inlc)}) (inrc:exp{is_closed (ELam inrc)}) =
   (fs_e == (match fs_cond with
            | Inl x -> fs_inlc x
            | Inr x -> fs_inrc x)) /\
@@ -1159,7 +852,7 @@ let equiv_case_prod_steps_pre (e e':closed_exp) (h:history) (lt:local_trace h) (
   ((a ^->!@ c) ⦂ (h, fs_inlc, ELam inlc)) /\
   ((b ^->!@ c) ⦂ (h, fs_inrc, ELam inrc))
 
-let equiv_case_prod_steps #e #e' #h #lt #a #b #c #fs_cond #fs_inlc #fs_inrc #fs_e #cond #inlc #inrc (sq:squash (equiv_case_prod_steps_pre e e' h lt a b c fs_cond fs_inlc fs_inrc fs_e cond inlc inrc)) : squash (exists (fs_r:get_Type c). c ∋ (h++lt, fs_r, e') /\ fs_beh fs_e h lt fs_r) =
+let helper_equiv_oprod_case_oval_steps #e #e' #h #lt #a #b #c #fs_cond #fs_inlc #fs_inrc #fs_e #cond #inlc #inrc (sq:squash (helper_equiv_oprod_case_oval_steps_pre e e' h lt a b c fs_cond fs_inlc fs_inrc fs_e cond inlc inrc)) : squash (exists (fs_r:get_Type c). c ∋ (h++lt, fs_r, e') /\ fs_beh fs_e h lt fs_r) =
   lem_forall_values_are_values (a ^+ b) h fs_cond;
   assert (forall cond' lt'. e_beh cond cond' h lt' ==> ((EInl? cond' \/ EInr? cond') /\ is_value cond'));
   FStar.Squash.bind_squash #(steps e e' h lt) () (fun sts ->
@@ -1194,8 +887,8 @@ let equiv_oprod_case_oval #g (#a #b #c:qType) (fs_cond:fs_oval g (a ^+ b)) (fs_i
   lem_fv_in_env_case g a b cond inlc inrc;
   lem_fv_in_env_lam g a inlc;
   lem_fv_in_env_lam g b inrc;
-  equiv_lam_prod fs_inlc inlc;
-  equiv_lam_prod fs_inrc inrc;
+  equiv_oval_lambda_oprod fs_inlc inlc;
+  equiv_oval_lambda_oprod fs_inrc inrc;
   introduce forall b' (s:gsub g b') fsG h. fsG `(∽) h` s ==> c ⪾ (h,
     (match fs_cond fsG with
     | Inl x -> fs_inlc (stack fsG x)
@@ -1221,22 +914,22 @@ let equiv_oprod_case_oval #g (#a #b #c:qType) (fs_cond:fs_oval g (a ^+ b)) (fs_i
         introduce e_beh e e' h lt /\ indexed_irred e' (h++lt) ==> (exists (fs_r:get_Type c). c ∋ (h++lt, fs_r, e') /\ fs_beh fs_e h lt fs_r) with _. begin
           assert ((a ^->!@ c) ⦂ (h, fs_inlc', ELam inlc));
           assert ((b ^->!@ c) ⦂ (h, fs_inrc', ELam inrc));
-          let steps_pre : squash (equiv_case_prod_steps_pre e e' h lt a b c fs_cond fs_inlc' fs_inrc' fs_e cond inlc inrc) = () in
+          let steps_pre : squash (helper_equiv_oprod_case_oval_steps_pre e e' h lt a b c fs_cond fs_inlc' fs_inrc' fs_e cond inlc inrc) = () in
           FStar.Squash.map_squash #_ #(squash (exists (fs_r:get_Type c). c ∋ (h++lt, fs_r, e') /\ fs_beh fs_e h lt fs_r)) steps_pre (fun steps_pre ->
-            equiv_case_prod_steps #e #e' #h #lt #a #b #c #fs_cond #fs_inlc' #fs_inrc' #fs_e #cond #inlc #inrc steps_pre)
+            helper_equiv_oprod_case_oval_steps #e #e' #h #lt #a #b #c #fs_cond #fs_inlc' #fs_inrc' #fs_e #cond #inlc #inrc steps_pre)
         end
       end
     end
   end
 #pop-options
 
-let equiv_oprod_openfile_steps_pre (e e':closed_exp) (h:history) (lt:local_trace h) (fs_fnm:bool) (fs_e:io (get_Type (qFileDescr ^+ qUnit))) (fnm:closed_exp) =
+let helper_equiv_oprod_openfile_oval_steps_pre (e e':closed_exp) (h:history) (lt:local_trace h) (fs_fnm:bool) (fs_e:io (get_Type (qFileDescr ^+ qUnit))) (fnm:closed_exp) =
   (fs_e == openfile fs_fnm) /\
   (e == EOpen fnm) /\
   (e_beh e e' h lt) /\
   (qBool ⦂ (h, fs_fnm, fnm))
 
-let equiv_oprod_openfile_steps #e #e' #h #lt #fs_fnm #fs_e #fnm (sq:squash (equiv_oprod_openfile_steps_pre e e' h lt fs_fnm fs_e fnm)) : squash (exists (fs_r:get_Type (qFileDescr ^+ qUnit)). (qFileDescr ^+ qUnit) ∋ (h++lt, fs_r, e') /\ fs_beh fs_e h lt fs_r) =
+let helper_equiv_oprod_openfile_oval_steps #e #e' #h #lt #fs_fnm #fs_e #fnm (sq:squash (helper_equiv_oprod_openfile_oval_steps_pre e e' h lt fs_fnm fs_e fnm)) : squash (exists (fs_r:get_Type (qFileDescr ^+ qUnit)). (qFileDescr ^+ qUnit) ∋ (h++lt, fs_r, e') /\ fs_beh fs_e h lt fs_r) =
   lem_forall_values_are_values qBool h fs_fnm;
   FStar.Squash.bind_squash #(steps e e' h lt) () (fun steps_e_e' ->
   let (fnm', (| lt1, lt' |)) = destruct_steps_eopen_str fnm e' h lt steps_e_e' in
@@ -1277,21 +970,21 @@ let equiv_oprod_openfile_oval #g (fs_fnm:fs_oval g qBool) (fnm:exp)
     introduce fsG `(∽) h` s ==> (qFileDescr ^+ qUnit) ⪾ (h, fs_e, e) with _. begin
       introduce forall (lt:local_trace h) (e':closed_exp). e_beh e e' h lt ==> (exists (fs_r:get_Type (qFileDescr ^+ qUnit)). (qFileDescr ^+ qUnit) ∋ (h++lt, fs_r, e') /\ fs_beh fs_e h lt fs_r) with begin
         introduce e_beh e e' h lt ==> (exists (fs_r:get_Type (qFileDescr ^+ qUnit)). (qFileDescr ^+ qUnit) ∋ (h++lt, fs_r, e') /\ fs_beh fs_e h lt fs_r) with _. begin
-        let steps_pre : squash (equiv_oprod_openfile_steps_pre e e' h lt fs_fnm fs_e fnm) = () in
+        let steps_pre : squash (helper_equiv_oprod_openfile_oval_steps_pre e e' h lt fs_fnm fs_e fnm) = () in
         FStar.Squash.map_squash #_ #(squash (exists (fs_r:get_Type (qFileDescr ^+ qUnit)). (qFileDescr ^+ qUnit) ∋ (h++lt, fs_r, e') /\ fs_beh fs_e h lt fs_r)) steps_pre (fun steps_pre ->
-        equiv_oprod_openfile_steps #e #e' #h #lt #fs_fnm #fs_e #fnm steps_pre)
+        helper_equiv_oprod_openfile_oval_steps #e #e' #h #lt #fs_fnm #fs_e #fnm steps_pre)
         end
       end
     end
   end
 
-let equiv_oprod_read_steps_pre (e e':closed_exp) (h:history) (lt:local_trace h) (fs_fd:get_Type qFileDescr) (fs_e:io (get_Type (qBool ^+ qUnit))) (fd:closed_exp) =
+let helper_equiv_oprod_read_oval_steps_pre (e e':closed_exp) (h:history) (lt:local_trace h) (fs_fd:get_Type qFileDescr) (fs_e:io (get_Type (qBool ^+ qUnit))) (fd:closed_exp) =
   (fs_e == read fs_fd) /\
   (e == ERead fd) /\
   (e_beh e e' h lt) /\
   (qFileDescr ⦂ (h, fs_fd, fd))
 
-let equiv_oprod_read_steps #e #e' #h #lt #fs_fd #fs_e #fd (sq:squash (equiv_oprod_read_steps_pre e e' h lt fs_fd fs_e fd)) : squash (exists (fs_r:get_Type (qBool ^+ qUnit)). (qBool ^+ qUnit) ∋ (h++lt, fs_r, e') /\ fs_beh fs_e h lt fs_r) =
+let helper_equiv_oprod_read_oval_steps #e #e' #h #lt #fs_fd #fs_e #fd (sq:squash (helper_equiv_oprod_read_oval_steps_pre e e' h lt fs_fd fs_e fd)) : squash (exists (fs_r:get_Type (qBool ^+ qUnit)). (qBool ^+ qUnit) ∋ (h++lt, fs_r, e') /\ fs_beh fs_e h lt fs_r) =
   lem_forall_values_are_values qFileDescr h fs_fd;
   FStar.Squash.bind_squash #(steps e e' h lt) () (fun steps_e_e' ->
   let (fd', (| lt1, lt' |)) = destruct_steps_eread_fd fd e' h lt steps_e_e' in
@@ -1340,15 +1033,15 @@ let equiv_oprod_read_oval #g (fs_fd:fs_oval g qFileDescr) (fd:exp)
     introduce fsG `(∽) h` s ==> (qBool ^+ qUnit) ⪾ (h, fs_e, e) with _. begin
       introduce forall (lt:local_trace h) (e':closed_exp). e_beh e e' h lt ==> (exists (fs_r:get_Type (qBool ^+ qUnit)). (qBool ^+ qUnit) ∋ (h++lt, fs_r, e') /\ fs_beh fs_e h lt fs_r) with begin
         introduce e_beh e e' h lt ==> (exists (fs_r:get_Type (qBool ^+ qUnit)). (qBool ^+ qUnit) ∋ (h++lt, fs_r, e') /\ fs_beh fs_e h lt fs_r) with _. begin
-        let steps_pre : squash (equiv_oprod_read_steps_pre e e' h lt fs_fd fs_e fd) = () in
+        let steps_pre : squash (helper_equiv_oprod_read_oval_steps_pre e e' h lt fs_fd fs_e fd) = () in
         FStar.Squash.map_squash #_ #(squash (exists (fs_r:get_Type (qBool ^+ qUnit)). (qBool ^+ qUnit) ∋ (h++lt, fs_r, e') /\ fs_beh fs_e h lt fs_r)) steps_pre (fun steps_pre ->
-        equiv_oprod_read_steps #e #e' #h #lt #fs_fd #fs_e #fd steps_pre)
+        helper_equiv_oprod_read_oval_steps #e #e' #h #lt #fs_fd #fs_e #fd steps_pre)
         end
       end
     end
   end
 
-let equiv_write_steps_pre (e e':closed_exp) (h:history) (lt:local_trace h) (fs_fd:file_descr) (fs_msg:bool) (fs_e:fs_prod (qUnit ^+ qUnit)) (fd msg:closed_exp) =
+let helper_equiv_oprod_write_oval_steps_pre (e e':closed_exp) (h:history) (lt:local_trace h) (fs_fd:file_descr) (fs_msg:bool) (fs_e:fs_prod (qUnit ^+ qUnit)) (fd msg:closed_exp) =
   (fs_e == write (fs_fd, fs_msg)) /\
   (e == (EWrite fd msg)) /\
   e_beh (EWrite fd msg) e' h lt /\
@@ -1356,7 +1049,7 @@ let equiv_write_steps_pre (e e':closed_exp) (h:history) (lt:local_trace h) (fs_f
   (forall (lt:local_trace h). qBool ⦂ (h++lt, fs_msg, msg))
 
 #push-options "--z3rlimit 10000"
-let equiv_write_steps #e #e' #h #lt #fs_fd #fs_msg #fs_e #fd #msg (sq:squash (equiv_write_steps_pre e e' h lt fs_fd fs_msg fs_e fd msg)) : squash (exists (fs_r:get_Type (qUnit ^+ qUnit)). (qUnit ^+ qUnit) ∋ (h++lt, fs_r, e') /\ fs_beh fs_e h lt fs_r) =
+let helper_equiv_oprod_write_oval_steps #e #e' #h #lt #fs_fd #fs_msg #fs_e #fd #msg (sq:squash (helper_equiv_oprod_write_oval_steps_pre e e' h lt fs_fd fs_msg fs_e fd msg)) : squash (exists (fs_r:get_Type (qUnit ^+ qUnit)). (qUnit ^+ qUnit) ∋ (h++lt, fs_r, e') /\ fs_beh fs_e h lt fs_r) =
   lem_forall_values_are_values qFileDescr h fs_fd;
   FStar.Squash.bind_squash #(steps e e' h lt) () (fun sts ->
   let (fd', (| lt1, lt' |)) = destruct_steps_ewrite_fd fd msg e' h lt sts in
@@ -1404,21 +1097,21 @@ let equiv_oprod_write_oval #g (fs_fd:fs_oval g qFileDescr) (fs_msg:fs_oval g qBo
       introduce forall (lt:local_trace h) (e':closed_exp). e_beh e e' h lt ==> (exists (fs_r:get_Type (qUnit ^+ qUnit)). (qUnit ^+ qUnit) ∋ (h++lt, fs_r, e') /\ fs_beh fs_e h lt fs_r) with begin
         introduce e_beh e e' h lt ==> (exists (fs_r:get_Type (qUnit ^+ qUnit)). (qUnit ^+ qUnit) ∋ (h++lt, fs_r, e') /\ fs_beh fs_e h lt fs_r) with _. begin
           lem_shift_type_value_environments h fsG s;
-          let steps_pre : squash (equiv_write_steps_pre e e' h lt fs_fd fs_msg fs_e fd msg) = () in
+          let steps_pre : squash (helper_equiv_oprod_write_oval_steps_pre e e' h lt fs_fd fs_msg fs_e fd msg) = () in
           FStar.Squash.map_squash #_ #(squash (exists (fs_r:get_Type (qUnit ^+ qUnit)). (qUnit ^+ qUnit) ∋ (h++lt, fs_r, e') /\ fs_beh fs_e h lt fs_r)) steps_pre (fun steps_pre ->
-          equiv_write_steps #e #e' #h #lt #fs_fd #fs_msg #fs_e #fd #msg steps_pre)
+          helper_equiv_oprod_write_oval_steps #e #e' #h #lt #fs_fd #fs_msg #fs_e #fd #msg steps_pre)
         end
       end
     end
   end
 
-let equiv_oprod_close_steps_pre (e e':closed_exp) (h:history) (lt:local_trace h) (fs_fd:get_Type qFileDescr) (fs_e:io (get_Type (qUnit ^+ qUnit))) (fd:closed_exp) =
+let helper_equiv_oprod_close_oval_steps_pre (e e':closed_exp) (h:history) (lt:local_trace h) (fs_fd:get_Type qFileDescr) (fs_e:io (get_Type (qUnit ^+ qUnit))) (fd:closed_exp) =
   (fs_e == close fs_fd) /\
   (e == EClose fd) /\
   (e_beh e e' h lt) /\
   (qFileDescr ⦂ (h, fs_fd, fd))
 
-let equiv_oprod_close_steps #e #e' #h #lt #fs_fd #fs_e #fd (sq:squash (equiv_oprod_close_steps_pre e e' h lt fs_fd fs_e fd)) : squash (exists (fs_r:get_Type (qUnit ^+ qUnit)). (qUnit ^+ qUnit) ∋ (h++lt, fs_r, e') /\ fs_beh fs_e h lt fs_r) =
+let helper_equiv_oprod_close_oval_steps #e #e' #h #lt #fs_fd #fs_e #fd (sq:squash (helper_equiv_oprod_close_oval_steps_pre e e' h lt fs_fd fs_e fd)) : squash (exists (fs_r:get_Type (qUnit ^+ qUnit)). (qUnit ^+ qUnit) ∋ (h++lt, fs_r, e') /\ fs_beh fs_e h lt fs_r) =
   lem_forall_values_are_values qFileDescr h fs_fd;
   FStar.Squash.bind_squash #(steps e e' h lt) () (fun steps_e_e' ->
   let (fd', (| lt1, lt' |)) = destruct_steps_eclose_fd fd e' h lt steps_e_e' in
@@ -1459,24 +1152,24 @@ let equiv_oprod_close_oval #g (fs_fd:fs_oval g qFileDescr) (fd:exp)
     introduce fsG `(∽) h` s ==> (qUnit ^+ qUnit) ⪾ (h, fs_e, e) with _. begin
       introduce forall (lt:local_trace h) (e':closed_exp). e_beh e e' h lt ==> (exists (fs_r:get_Type (qUnit ^+ qUnit)). (qUnit ^+ qUnit) ∋ (h++lt, fs_r, e') /\ fs_beh fs_e h lt fs_r) with begin
         introduce e_beh e e' h lt ==> (exists (fs_r:get_Type (qUnit ^+ qUnit)). (qUnit ^+ qUnit) ∋ (h++lt, fs_r, e') /\ fs_beh fs_e h lt fs_r) with _. begin
-        let steps_pre : squash (equiv_oprod_close_steps_pre e e' h lt fs_fd fs_e fd) = () in
+        let steps_pre : squash (helper_equiv_oprod_close_oval_steps_pre e e' h lt fs_fd fs_e fd) = () in
         FStar.Squash.map_squash #_ #(squash (exists (fs_r:get_Type (qUnit ^+ qUnit)). (qUnit ^+ qUnit) ∋ (h++lt, fs_r, e') /\ fs_beh fs_e h lt fs_r)) steps_pre (fun steps_pre ->
-        equiv_oprod_close_steps #e #e' #h #lt #fs_fd #fs_e #fd steps_pre)
+        helper_equiv_oprod_close_oval_steps #e #e' #h #lt #fs_fd #fs_e #fd steps_pre)
         end
       end
     end
   end
 
 let equiv_oprod_unit g : Lemma (fs_oprod_return_val g qUnit () ≋ EUnit) =
-  equiv_unit g;
+  equiv_oval_unit g;
   equiv_oprod_return (fs_oval_return g qUnit ()) EUnit
 
 let equiv_oprod_true g : Lemma (fs_oprod_return_val g qBool true ≋ ETrue) =
-  equiv_true g;
+  equiv_oval_true g;
   equiv_oprod_return (fs_oval_return g qBool true) ETrue
 
 let equiv_oprod_false g : Lemma (fs_oprod_return_val g qBool false ≋ EFalse) =
-  equiv_false g;
+  equiv_oval_false g;
   equiv_oprod_return (fs_oval_return g qBool false) EFalse
 
 let equiv_oprod_if #g
@@ -1489,11 +1182,11 @@ let equiv_oprod_if #g
   admit ()
 
 let equiv_oprod_file_descr g fd : Lemma (fs_oprod_return_val g qFileDescr fd ≋ EFileDescr fd) =
-  equiv_file_descr g fd;
+  equiv_oval_file_descr g fd;
   equiv_oprod_return (fs_oval_return g qFileDescr fd) (EFileDescr fd)
 
 let equiv_oprod_var g (x:var{Some? (g x)}) : Lemma (fs_oprod_var g x ≋ EVar x) =
-  equiv_var g x;
+  equiv_oval_var g x;
   equiv_oprod_return (fs_oval_var g x) (EVar x)
 
 let equiv_oprod_app_steps_pre' (e e':closed_exp) (h:history) (lt:local_trace h) (a b:qType) (fs_x':(get_Type (a ^->!@ b)) -> io (get_Type b)) (fs_f:io (get_Type (a ^->!@ b))) (fs_e':io (get_Type b)) (f x:exp) =
@@ -1545,7 +1238,7 @@ let equiv_oprod_lambda #g (#t1:qType) (#t2:qType)
     (requires fs_body ≋ body)
     (ensures fs_oprod_lambda fs_body ≋ (ELam body))
   =
-  equiv_lam_prod #g #t1 #t2 fs_body body;
+  equiv_oval_lambda_oprod #g #t1 #t2 fs_body body;
   equiv_oprod_return (fs_oval_lambda_oprod fs_body) (ELam body)
 
 let equiv_oprod_inl #g (t1 t2:qType) (fs_e:fs_oprod g t1) (e:exp)
