rupicola/io/Compilation.fsti
@@ -5,18 +5,21 @@ open FStar.Tactics
 open STLC
 open QTyp
 open QExp
-open ExpRel
+open LogRelSourceTarget
+open LogRelTargetSource
 
 val compile #g #a (#s:fs_oval g a) (qs:g ⊢ s) : exp
 
-val lem_compile_empty_closed #a (#s:fs_oval empty a) (qs:empty ⊢ s) : Lemma (is_closed (compile qs))
-
-val compile_closed (#a:qType) (#s:get_Type a) (qs:a ⊩ s) : closed_exp
-val compile_equiv #g (#a:qType) (#s:fs_oval g a) (qs:g ⊢ s)
+val lem_compile_equiv #g (#a:qType) (#s:fs_oval g a) (qs:g ⊢ s)
   : Lemma (ensures (s ≈ (compile qs))) (decreases qs)
 
-val compile_closed_equiv (#a:qType) (#s:get_Type a) (qs:a ⊩ s)
-  : Lemma (ensures (forall h. a ⦂ (h, s, compile_closed qs)))
+val lem_compile_closed_arrow_is_elam (#a #b:qType) (#s:fs_val (a ^->!@ b)) (qs: (a ^->!@ b) ⊩ s)
+  : Lemma (ELam? (compile qs))
 
-val lemma_compile_closed_arrow_is_elam (#a #b:qType) (#s:fs_val (a ^->!@ b)) (qs: (a ^->!@ b) ⊩ s)
-  : Lemma (ELam? (compile_closed qs))
+val lem_compile_closed_valid (#a:qType) (#s:fs_val a) (qs:a ⊩ s)
+  : Lemma (ensures (
+    is_closed (compile qs) /\
+    is_value (compile qs) /\
+    valid_in_val s (compile qs) /\
+    (forall hist. a ∈ (hist, s, compile qs))
+    ))
